Require commit's rel, cur, and acq are in order

src/lang/Commit.v
@@ -17,26 +17,28 @@ Set Implicit Arguments.
 
 Module Commit <: JoinableType.
   Structure t_ := mk {
-    current: Capability.t;
-    released: LocFun.t Capability.t;
-    acquirable: Capability.t;
+    rel: LocFun.t Capability.t;
+    cur: Capability.t;
+    acq: Capability.t;
   }.
   Definition t := t_.
 
-  Definition elt: t := mk Capability.elt (LocFun.init Capability.elt) Capability.elt.
+  Definition elt: t := mk (LocFun.init Capability.elt) Capability.elt Capability.elt.
 
   Inductive wf (commit:t): Prop :=
   | wf_intro
-      (CURRENT: Capability.wf commit.(current))
-      (RELEASED: forall loc, Capability.wf (commit.(released) loc))
-      (ACQUIRABLE: Capability.wf commit.(acquirable))
+      (REL: forall loc, Capability.wf (commit.(rel) loc))
+      (CUR: Capability.wf commit.(cur))
+      (ACQ: Capability.wf commit.(acq))
+      (REL_CUR: forall loc, Capability.le (commit.(rel) loc) commit.(cur))
+      (CUR_ACQ: Capability.le commit.(cur) commit.(acq))
   .
 
   Inductive closed (commit:t) (mem:Memory.t): Prop :=
   | closed_intro
-      (CURRENT: Memory.closed_capability commit.(current) mem)
-      (RELEASED: forall loc, Memory.closed_capability (commit.(released) loc) mem)
-      (ACQUIRABLE: Memory.closed_capability commit.(acquirable) mem)
+      (REL: forall loc, Memory.closed_capability (commit.(rel) loc) mem)
+      (CUR: Memory.closed_capability commit.(cur) mem)
+      (ACQ: Memory.closed_capability commit.(acq) mem)
   .
 
   Lemma future_closed
@@ -52,9 +54,9 @@ Module Commit <: JoinableType.
 
   Inductive le_ (lhs rhs:t): Prop :=
   | le_intro
-      (CURRENT: Capability.le lhs.(current) rhs.(current))
-      (RELEASED: forall (loc:Loc.t), Capability.le (LocFun.find loc lhs.(released)) (LocFun.find loc rhs.(released)))
-      (ACQUIRABLE: Capability.le lhs.(acquirable) rhs.(acquirable))
+      (REL: forall (loc:Loc.t), Capability.le (LocFun.find loc lhs.(rel)) (LocFun.find loc rhs.(rel)))
+      (CUR: Capability.le lhs.(cur) rhs.(cur))
+      (ACQ: Capability.le lhs.(acq) rhs.(acq))
   .
   Definition le := le_.
 
@@ -67,39 +69,39 @@ Module Commit <: JoinableType.
   Qed.
 
   Definition join (lhs rhs:t): t :=
-    mk (Capability.join lhs.(current) rhs.(current))
-       (fun loc => Capability.join (lhs.(released) loc) (rhs.(released) loc))
-       (Capability.join lhs.(acquirable) rhs.(acquirable)).
+    mk (fun loc => Capability.join (lhs.(rel) loc) (rhs.(rel) loc))
+       (Capability.join lhs.(cur) rhs.(cur))
+       (Capability.join lhs.(acq) rhs.(acq)).
 
   Lemma join_comm lhs rhs: join lhs rhs = join rhs lhs.
   Proof.
     unfold join. f_equal.
-    - apply Capability.join_comm.
     - extensionality loc. apply Capability.join_comm.
+    - apply Capability.join_comm.
     - apply Capability.join_comm.
   Qed.
 
   Lemma join_assoc a b c: join (join a b) c = join a (join b c).
   Proof.
     unfold join. s. f_equal.
-    - apply Capability.join_assoc.
     - extensionality loc. apply Capability.join_assoc.
+    - apply Capability.join_assoc.
     - apply Capability.join_assoc.
   Qed.
 
   Lemma join_l lhs rhs: le lhs (join lhs rhs).
   Proof.
     econs.
-    - apply Capability.join_l.
     - i. apply Capability.join_l.
+    - apply Capability.join_l.
     - apply Capability.join_l.
   Qed.
 
   Lemma join_r lhs rhs: le rhs (join lhs rhs).
   Proof.
     econs.
-    - apply Capability.join_r.
     - i. apply Capability.join_r.
+    - apply Capability.join_r.
     - apply Capability.join_r.
   Qed.
 
@@ -109,8 +111,8 @@ Module Commit <: JoinableType.
     le (join lhs rhs) o.
   Proof.
     inv LHS. inv RHS. econs.
-    - apply Capability.join_spec; eauto.
     - i. apply Capability.join_spec; eauto.
+    - apply Capability.join_spec; eauto.
     - apply Capability.join_spec; eauto.
   Qed.
 
@@ -118,15 +120,15 @@ Module Commit <: JoinableType.
             (commit1:t) (loc:Loc.t) (ts:Time.t) (released:Capability.t) (ord:Ordering.t)
             (commit2:t): Prop :=
   | read_intro
-      (MONOTONE: le commit1 commit2)
-      (ACQUIRABLE: Capability.le released commit2.(acquirable))
-      (UR1: Time.le (commit1.(current).(Capability.ur) loc) ts)
+      (MON: le commit1 commit2)
+      (ACQ: Capability.le released commit2.(acq))
+      (UR1: Time.le (commit1.(cur).(Capability.ur) loc) ts)
       (RW1: Ordering.le Ordering.relaxed ord ->
-            Time.le (commit1.(current).(Capability.rw) loc) ts)
-      (RW2: Time.le ts (commit2.(current).(Capability.rw) loc))
+            Time.le (commit1.(cur).(Capability.rw) loc) ts)
+      (RW2: Time.le ts (commit2.(cur).(Capability.rw) loc))
       (RA: Ordering.le Ordering.acqrel ord ->
-           Capability.le released commit2.(current))
-      (WF_RELEASED: Capability.wf released)
+           Capability.le released commit2.(cur))
+      (WF_REL: Capability.wf released)
       (WF: Commit.wf commit2)
   .
 
@@ -134,16 +136,16 @@ Module Commit <: JoinableType.
             (commit1:t) (loc:Loc.t) (ts:Time.t) (released:Capability.t) (ord:Ordering.t)
             (commit2:t): Prop :=
   | write_intro
-      (MONOTONE: le commit1 commit2)
-      (RELEASED: Time.le (released.(Capability.rw) loc) ts)
-      (RW1: Time.le (commit1.(current).(Capability.rw) loc) ts)
-      (RW2: Time.le ts (commit2.(current).(Capability.ur) loc))
-      (REL1: Capability.le (commit1.(Commit.released) loc) released)
-      (REL2: Capability.le released (commit2.(Commit.released) loc))
+      (MON: le commit1 commit2)
+      (REL: Time.le (released.(Capability.rw) loc) ts)
+      (RW1: Time.le (commit1.(cur).(Capability.rw) loc) ts)
+      (RW2: Time.le ts (commit2.(cur).(Capability.ur) loc))
+      (REL1: Capability.le (commit1.(Commit.rel) loc) released)
+      (REL2: Capability.le released (commit2.(Commit.rel) loc))
       (RA: Ordering.le Ordering.acqrel ord ->
-           Capability.le commit1.(Commit.current) released /\
+           Capability.le commit1.(Commit.cur) released /\
            Time.le ts (released.(Capability.rw) loc))
-      (WF_RELEASED: Capability.wf released)
+      (WF_REL: Capability.wf released)
       (WF: Commit.wf commit2)
   .
 
@@ -151,9 +153,9 @@ Module Commit <: JoinableType.
             (commit1:t) (ord:Ordering.t)
             (commit2:t): Prop :=
   | read_fence_intro
-      (MONOTONE: le commit1 commit2)
+      (MON: le commit1 commit2)
       (RA: Ordering.le Ordering.acqrel ord ->
-           Capability.le commit1.(Commit.acquirable) commit2.(Commit.current))
+           Capability.le commit1.(Commit.acq) commit2.(Commit.cur))
       (WF: Commit.wf commit2)
   .
 
@@ -161,11 +163,9 @@ Module Commit <: JoinableType.
             (commit1:t) (ord:Ordering.t)
             (commit2:t): Prop :=
   | write_fence_intro
-      (MONOTONE: le commit1 commit2)
-      (RLX: Ordering.le Ordering.relaxed ord -> TimeMap.le commit1.(current).(Capability.rw) commit2.(current).(Capability.ur))
+      (MON: le commit1 commit2)
       (RA: Ordering.le Ordering.acqrel ord ->
-           forall loc, TimeMap.le commit1.(current).(Capability.rw) (commit2.(released) loc).(Capability.ur) /\
-                  Capability.le commit1.(Commit.current) (commit2.(Commit.released) loc))
+           forall loc, Capability.le commit1.(Commit.cur) (commit2.(Commit.rel) loc))
       (WF: Commit.wf commit2)
   .
 End Commit.
@@ -212,11 +212,10 @@ Module CommitFacts.
   Lemma wf_get
         loc commit1 mem
         (CLOSED: Commit.closed commit1 mem):
-    exists ts msg,
-      Time.le (commit1.(Commit.current).(Capability.rw) loc) ts /\
-      Memory.get loc ts mem = Some msg.
+    exists msg,
+      Memory.get loc (commit1.(Commit.cur).(Capability.rw) loc) mem = Some msg.
   Proof.
-    inversion CLOSED. inv CURRENT.
+    inversion CLOSED. inv CUR.
     specialize (RW loc). des. eauto.
   Qed.
 
@@ -262,9 +261,6 @@ Module CommitFacts.
     i. inv PR. econs; auto.
     - etrans; [apply LE|]. auto.
     - etrans; [apply LE|]. auto.
-    - i. splits.
-      + etrans; [apply LE|]. apply RA. auto.
-      + etrans; [apply LE|]. apply RA. auto.
   Qed.
 
   Lemma read_mon2
@@ -329,28 +325,24 @@ Module CommitFacts.
   Proof.
     inv FENCE. econs; auto.
     - etrans; [|apply LE]. auto.
-    - etrans; [|apply LE].
-      apply RLX. etrans; eauto.
-    - i. exploit RA.
-      { etrans; eauto. }
-      i. des. splits.
-      + etrans; [|apply LE]. eauto.
-      + etrans; [|apply LE]. eauto.
+    - etrans; [|apply LE]. apply RA. etrans; eauto.
   Qed.
 
   Definition read_min
              loc ts released ord commit: Commit.t :=
-    (Commit.mk (Capability.join_if
+    (Commit.mk commit.(Commit.rel)
+               (Capability.join_if
                   (Ordering.le Ordering.acqrel ord)
                   released
-                  (Capability.incr_rw loc ts commit.(Commit.current)))
-               commit.(Commit.released)
-               (Capability.join released commit.(Commit.acquirable))).
+                  (Capability.incr_rw loc ts commit.(Commit.cur)))
+               (Capability.join
+                  released
+                  (Capability.incr_rw loc ts commit.(Commit.acq)))).
 
   Lemma read_min_spec
         loc ts released ord commit
-        (UR: Time.le (commit.(Commit.current).(Capability.ur) loc) ts)
-        (RW: Ordering.le Ordering.relaxed ord -> Time.le (commit.(Commit.current).(Capability.rw) loc) ts)
+        (UR: Time.le (commit.(Commit.cur).(Capability.ur) loc) ts)
+        (RW: Ordering.le Ordering.relaxed ord -> Time.le (commit.(Commit.cur).(Capability.rw) loc) ts)
         (WF1: Commit.wf commit)
         (WF_RELEASED: Capability.wf released):
     Commit.read commit loc ts released ord (read_min loc ts released ord commit).
@@ -358,162 +350,184 @@ Module CommitFacts.
     unfold read_min. econs; tac.
     - econs; tac; try reflexivity.
       unfold Capability.join_if. condtac; tac.
-      etrans; [|apply Capability.join_r]. tac.
+      + rewrite <- Capability.join_r. tac.
+      + rewrite <- Capability.join_r. tac.
     - unfold Capability.join_if. condtac; tac.
       + etrans; [|apply TimeMap.join_r].
         apply TimeMap.incr_ts.
       + apply TimeMap.incr_ts.
     - unfold Capability.join_if. condtac; tac.
     - econs; s.
+      + apply WF1.
       + apply Capability.join_if_wf; auto.
         apply Capability.incr_rw_wf; auto.
         apply WF1.
-      + apply WF1.
       + apply Capability.join_wf; auto.
+        apply Capability.incr_rw_wf; auto.
         apply WF1.
+      + i. unfold Capability.join_if. condtac; tac.
+        * etrans; [apply WF1|].
+          rewrite <- Capability.join_r. tac.
+        * etrans; [apply WF1|]. tac.
+      + unfold Capability.join_if. condtac; tac.
+        * etrans; [apply WF1|].
+          rewrite <- Capability.join_r. tac.
+        * etrans; [|apply Time.join_r].
+          apply TimeMap.incr_ts.
+        * etrans; [|apply Time.join_r].
+          apply TimeMap.incr_ts.
+        * etrans; [apply WF1|].
+          rewrite <- Capability.join_r. tac.
+        * etrans; [|apply Time.join_r].
+          apply TimeMap.incr_ts.
+        * etrans; [|apply Time.join_r].
+          apply TimeMap.incr_ts.
   Qed.
 
   Lemma read_min_min
         loc ts released ord commit1 commit2
-        (COMMIT2: Commit.read commit1 loc ts released ord commit2)
-        (WF2: Commit.wf commit2):
+        (COMMIT2: Commit.read commit1 loc ts released ord commit2):
     Commit.le (read_min loc ts released ord commit1) commit2.
   Proof.
     inv COMMIT2. unfold read_min. econs; tac.
-    - apply MONOTONE.
-    - rewrite RW2. apply WF2.
-    - apply MONOTONE.
-    - apply MONOTONE.
+    - apply MON.
+    - apply MON.
+    - rewrite RW2. apply WF.
+    - apply MON.
+    - etrans; eauto. apply WF.
+    - etrans; eauto. etrans; apply WF.
   Qed.
 
   Definition write_min
              loc ts released commit: Commit.t :=
-    (Commit.mk (Capability.incr_ur loc ts commit.(Commit.current))
-               (LocFun.add loc released commit.(Commit.released))
-               commit.(Commit.acquirable)).
+    (Commit.mk (LocFun.add loc released commit.(Commit.rel))
+               (Capability.join released (Capability.incr_ur loc ts commit.(Commit.cur)))
+               (Capability.join released (Capability.incr_ur loc ts commit.(Commit.acq)))).
 
   Lemma write_min_spec
         loc ts released ord commit
         (RELEASED: Time.le (released.(Capability.rw) loc) ts)
-        (RW1: Time.le (commit.(Commit.current).(Capability.rw) loc) ts)
-        (REL1: Capability.le (commit.(Commit.released) loc) released)
+        (RW1: Time.le (commit.(Commit.cur).(Capability.rw) loc) ts)
+        (REL1: Capability.le (commit.(Commit.rel) loc) released)
         (RA: Ordering.le Ordering.acqrel ord ->
-             Capability.le commit.(Commit.current) released /\
+             Capability.le commit.(Commit.cur) released /\
              Time.le ts (released.(Capability.rw) loc))
         (WF1: Commit.wf commit)
         (WF_RELEASED: Capability.wf released):
     Commit.write commit loc ts released ord (write_min loc ts released commit).
   Proof.
     econs; tac.
-    - econs; tac; try reflexivity.
-      unfold LocFun.add, LocFun.find.
-      condtac; tac. reflexivity.
-    - apply TimeMap.incr_ts.
+    - econs; tac.
+      + unfold LocFun.add, LocFun.find. condtac; tac. reflexivity.
+      + rewrite <- Capability.join_r. tac.
+      + rewrite <- Capability.join_r. tac.
+    - etrans; [|apply TimeMap.join_r].
+      apply TimeMap.incr_ts.
     - unfold LocFun.add, LocFun.find.
       condtac; [|congruence]. reflexivity.
     - econs; try apply WF1; tac.
-      + apply Capability.incr_ur_wf. apply WF1.
-      + unfold LocFun.add, LocFun.find.
-        condtac; tac. apply WF1.
+      + unfold LocFun.add, LocFun.find. condtac; auto. apply WF1.
+      + apply Capability.join_wf; auto.
+        apply Capability.incr_ur_wf. apply WF1.
+      + apply Capability.join_wf; auto.
+        apply Capability.incr_ur_wf. apply WF1.
+      + unfold LocFun.add, LocFun.find. condtac; tac.
+        rewrite <- Capability.join_r.
+        rewrite <- Capability.incr_ur_le.
+        apply WF1.
+      + rewrite <- Capability.join_r.
+        rewrite <- Capability.incr_ur_le.
+        apply WF1.
+      + etrans; [|apply TimeMap.join_r].
+        apply TimeMap.incr_ts.
+      + etrans; [|apply TimeMap.join_r].
+        apply TimeMap.incr_ts.
+      + etrans; [|apply TimeMap.join_r].
+        apply TimeMap.incr_ts.
   Qed.
 
   Lemma write_min_min
         loc ts released ord commit1 commit2
-        (COMMIT2: Commit.write commit1 loc ts released ord commit2)
-        (WF2: Commit.wf commit2):
+        (COMMIT2: Commit.write commit1 loc ts released ord commit2):
     Commit.le (write_min loc ts released commit1) commit2.
   Proof.
-    i. inv COMMIT2. econs; tac; try apply MONOTONE.
-    - rewrite RW2. apply WF2.
-    - rewrite RW2. etrans; apply WF2.
+    i. inv COMMIT2.
+    econs; tac;
+      (try by apply MON);
+      (try by etrans; eauto; apply WF).
     - unfold LocFun.add, LocFun.find. condtac; tac.
-      apply MONOTONE.
+      apply MON.
+    - rewrite RW2. inv WF. etrans; apply CUR.
+    - rewrite REL2. etrans; apply WF.
+    - rewrite RW2. etrans; apply WF.
+    - rewrite RW2. etrans; [apply WF|].
+      inv WF. etrans; apply ACQ.
   Qed.
 
   Definition read_fence_min
              ord commit: Commit.t :=
-    Commit.mk (Capability.join_if
-                 (Ordering.le Ordering.acqrel ord)
-                 commit.(Commit.acquirable)
-                 commit.(Commit.current))
-              commit.(Commit.released)
-              commit.(Commit.acquirable).
+    Commit.mk commit.(Commit.rel)
+              (if Ordering.le Ordering.acqrel ord
+               then commit.(Commit.acq)
+               else commit.(Commit.cur))
+              commit.(Commit.acq).
 
   Lemma read_fence_min_spec
         ord commit
         (WF1: Commit.wf commit):
     Commit.read_fence commit ord (read_fence_min ord commit).
   Proof.
-    unfold read_fence_min. econs; tac.
-    - econs; tac; try reflexivity.
-      unfold Capability.join_if. condtac; tac. reflexivity.
-    - rewrite H. s. apply Capability.join_l.
-    - econs; try apply WF1. s.
-      apply Capability.join_if_wf; apply WF1.
+    unfold read_fence_min. econs; tac; try apply WF1.
+    - econs; tac; try reflexivity. apply WF1.
+    - reflexivity.
+    - econs; s; try apply WF1.
+      + condtac; try apply WF1.
+      + i. condtac; try apply WF1.
+        etrans; apply WF1.
+      + condtac; try apply WF1. reflexivity.
   Qed.
 
   Lemma read_fence_min_min
         ord commit1 commit2
+        (WF1: Commit.wf commit1)
         (COMMIT2: Commit.read_fence commit1 ord commit2):
     Commit.le (read_fence_min ord commit1) commit2.
   Proof.
-    inv COMMIT2. unfold read_fence_min. econs; tac; try apply MONOTONE.
+    inv COMMIT2. unfold read_fence_min. econs; tac; try apply MON.
+    condtac; try apply MON. eauto.
   Qed.
 
   Definition write_fence_min
              ord commit: Commit.t :=
-    Commit.mk (Capability.join_if
-                 (Ordering.le Ordering.relaxed ord)
-                 (Capability.mk commit.(Commit.current).(Capability.rw)
-                                commit.(Commit.current).(Capability.rw)
-                                commit.(Commit.current).(Capability.sc))
-                 commit.(Commit.current))
-              (fun loc =>
-                 Capability.join_if
-                   (Ordering.le Ordering.acqrel ord)
-                   (Capability.mk commit.(Commit.current).(Capability.rw)
-                                  commit.(Commit.current).(Capability.rw)
-                                  commit.(Commit.current).(Capability.sc))
-                   (commit.(Commit.released) loc))
-              commit.(Commit.acquirable).
+    Commit.mk (fun loc =>
+                 if Ordering.le Ordering.acqrel ord
+                 then commit.(Commit.cur)
+                 else (commit.(Commit.rel) loc))
+              commit.(Commit.cur)
+              commit.(Commit.acq).
 
   Lemma write_fence_min_spec
         ord commit
         (WF1: Commit.wf commit):
     Commit.write_fence commit ord (write_fence_min ord commit).
   Proof.
-    econs; tac.
+    econs; tac; try reflexivity.
     - econs; tac; try reflexivity.
-      + unfold Capability.join_if. condtac; tac. reflexivity.
-      + unfold LocFun.find.
-        unfold Capability.join_if. condtac; tac. reflexivity.
-    - unfold Capability.join_if. condtac; tac.
-      apply TimeMap.join_l.
-    - unfold Capability.join_if. condtac; tac. splits.
-      + apply TimeMap.join_l.
-      + etrans; [|apply Capability.join_l].
-        econs; try reflexivity.
-        apply WF1.
+      condtac; try reflexivity.
+      apply WF1.
     - econs; tac; try apply WF1.
-      + apply Capability.join_if_wf; try apply WF1.
-        econs; s; try apply WF1. reflexivity.
-      + apply Capability.join_if_wf; try apply WF1.
-        econs; try apply WF1. reflexivity.
-  Qed.        
+      + condtac; apply WF1.
+      + condtac; try apply WF1. reflexivity.
+  Qed.
 
   Lemma write_fence_min_min
         ord commit1 commit2
+        (WF1: Commit.wf commit1)
         (COMMIT2: Commit.write_fence commit1 ord commit2):
     Commit.le (write_fence_min ord commit1) commit2.
   Proof.
-    inv COMMIT2. unfold write_fence_min. econs; tac; try apply MONOTONE.
-    - econs; tac; try apply MONOTONE. eauto.
-    - unfold LocFun.find.
-      unfold Capability.join_if. condtac; tac; try apply MONOTONE.
-      econs; s.
-      + apply RA. auto.
-      + apply RA. auto.
-      + apply RA. auto.
+    inv COMMIT2. unfold write_fence_min. econs; tac; try apply MON.
+    condtac; try apply MON. eauto.
   Qed.
 End CommitFacts.
 
